more symmetrical definition

Weidenbach_Book/IsaSAT_Arena.thy
@@ -2017,16 +2017,16 @@ lemma isa_get_clause_LBD_code[sepref_fr_rules]:
 paragraph \<open>Saved position\<close>
 
 definition get_saved_pos :: \<open>arena \<Rightarrow> nat \<Rightarrow> nat\<close> where
-  \<open>get_saved_pos arena C =  xarena_pos (arena ! (C - POS_SHIFT))\<close>
+  \<open>get_saved_pos arena C =  xarena_pos (arena ! (C - POS_SHIFT)) + 2\<close>
 
 definition get_saved_pos_pre where
   \<open>get_saved_pos_pre arena C \<longleftrightarrow> arena_is_valid_clause_idx arena C \<and>
       arena_length arena C > 5\<close>
 
-definition isa_get_saved_pos :: \<open>uint32 list \<Rightarrow> nat \<Rightarrow> uint32 nres\<close> where
+definition isa_get_saved_pos :: \<open>uint32 list \<Rightarrow> nat \<Rightarrow> uint64 nres\<close> where
   \<open>isa_get_saved_pos arena C = do {
       ASSERT(C - POS_SHIFT < length arena \<and> C \<ge> POS_SHIFT);
-      RETURN (arena ! (C - POS_SHIFT))
+      RETURN (uint64_of_uint32 (arena ! (C - POS_SHIFT)) + two_uint64)
   }\<close>
 
 lemma arena_get_pos_conv:
@@ -2038,9 +2038,15 @@ lemma arena_get_pos_conv:
   shows
     \<open>j - POS_SHIFT < length arena\<close> (is ?le) and
     \<open>POS_SHIFT \<le> j\<close> (is ?ge) and
-    \<open>(a ! (j - POS_SHIFT),
-        xarena_pos (arena ! (j - POS_SHIFT)))
-       \<in> uint32_nat_rel\<close>
+    \<open>(uint64_of_uint32 (a ! (j - POS_SHIFT)) + two_uint64,
+        Suc (Suc (xarena_pos (arena ! (j - POS_SHIFT)))))
+       \<in> uint64_nat_rel\<close> (is ?rel) and
+    \<open>nat_of_uint64
+        (uint64_of_uint32
+          (a ! (j - POS_SHIFT)) +
+         two_uint64) =
+       Suc (Suc (xarena_pos
+                  (arena ! (j - POS_SHIFT))))\<close> (is ?eq')
 proof -
   have j_le: \<open>j < length arena\<close> and
     length: \<open>length (N \<propto> j) = arena_length arena j\<close> and
@@ -2062,17 +2068,29 @@ proof -
          (arena ! (j - POS_SHIFT)))
        \<in> uint32_nat_rel O arena_el_rel\<close>
     by (rule param_nth[OF _ _ a]) (use j_le in auto)
-  then show \<open>(a ! (j - POS_SHIFT),
-        xarena_pos (arena ! (j - POS_SHIFT)))
-       \<in> uint32_nat_rel\<close>
-    using lbd by (cases \<open>arena ! (j - POS_SHIFT)\<close>) (auto simp: arena_el_rel_def)
+  moreover have \<open>Suc (Suc (nat_of_uint32 (a ! (j - POS_SHIFT)))) \<le> uint64_max\<close>
+    using nat_of_uint32_le_uint32_max[of \<open>a ! (j - POS_SHIFT)\<close>]
+    unfolding uint64_max_def uint32_max_def
+    by auto
+  ultimately show ?rel
+    using lbd apply (cases \<open>arena ! (j - POS_SHIFT)\<close>) 
+    by (auto simp: arena_el_rel_def
+      uint64_nat_rel_def br_def two_uint64_def uint32_nat_rel_def nat_of_uint64_add
+      uint64_of_uint32_def nat_of_uint64_add 
+      nat_of_uint64_uint64_of_nat_id nat_of_uint32_le_uint64_max)
+  then show ?eq'
+    using lbd \<open>?rel\<close> apply (cases \<open>arena ! (j - POS_SHIFT)\<close>) 
+    by (auto simp: arena_el_rel_def
+      uint64_nat_rel_def br_def two_uint64_def uint32_nat_rel_def nat_of_uint64_add
+      uint64_of_uint32_def nat_of_uint64_add 
+      nat_of_uint64_uint64_of_nat_id nat_of_uint32_le_uint64_max)
 qed
 
 lemma isa_get_saved_pos_get_saved_pos:
   \<open>(uncurry isa_get_saved_pos, uncurry (RETURN oo get_saved_pos)) \<in>
     [uncurry get_saved_pos_pre]\<^sub>f
      \<langle>uint32_nat_rel O arena_el_rel\<rangle>list_rel \<times>\<^sub>f nat_rel \<rightarrow> 
-    \<langle>uint32_nat_rel\<rangle>nres_rel\<close>
+    \<langle>uint64_nat_rel\<rangle>nres_rel\<close>
   by (intro frefI nres_relI)
     (auto simp: isa_get_saved_pos_def get_saved_pos_def arena_get_lbd_conv
       arena_is_valid_clause_idx_def arena_get_pos_conv
@@ -2084,16 +2102,49 @@ lemma [sepref_fr_rules]:
   \<open>(uncurry0 (return 5), uncurry0 (RETURN POS_SHIFT)) \<in> unit_assn\<^sup>k \<rightarrow>\<^sub>a nat_assn\<close>
   by sepref_to_hoare (sep_auto simp: SHIFTS_def)
 
-sepref_definition isa_get_saved_pos_code
+sepref_definition isa_get_saved_pos_fast_code
   is \<open>uncurry isa_get_saved_pos\<close>
-  :: \<open>(arl_assn uint32_assn)\<^sup>k *\<^sub>a nat_assn\<^sup>k \<rightarrow>\<^sub>a uint32_assn\<close>
+  :: \<open>(arl_assn uint32_assn)\<^sup>k *\<^sub>a nat_assn\<^sup>k \<rightarrow>\<^sub>a uint64_assn\<close>
+  supply sum_uint64_assn[sepref_fr_rules]
   unfolding isa_get_saved_pos_def
   by sepref
 
-lemma get_saved_pos_code[sepref_fr_rules]:
+lemma get_saved_pos_code:
+  \<open>(uncurry isa_get_saved_pos_fast_code, uncurry (RETURN \<circ>\<circ> get_saved_pos))
+     \<in> [uncurry get_saved_pos_pre]\<^sub>a arena_assn\<^sup>k *\<^sub>a nat_assn\<^sup>k \<rightarrow> uint64_nat_assn\<close>
+  using isa_get_saved_pos_fast_code.refine[FCOMP isa_get_saved_pos_get_saved_pos]
+  unfolding hr_comp_assoc[symmetric] list_rel_compp status_assn_alt_def uncurry_def
+  by (auto simp add: arl_assn_comp update_lbd_pre_def)
+
+definition isa_get_saved_pos' :: \<open>uint32 list \<Rightarrow> nat \<Rightarrow> nat nres\<close> where
+  \<open>isa_get_saved_pos' arena C = do {
+      pos \<leftarrow> isa_get_saved_pos arena C;
+      RETURN (nat_of_uint64 pos)
+  }\<close>
+
+
+sepref_definition isa_get_saved_pos_code
+  is \<open>uncurry isa_get_saved_pos'\<close>
+  :: \<open>(arl_assn uint32_assn)\<^sup>k *\<^sub>a nat_assn\<^sup>k \<rightarrow>\<^sub>a nat_assn\<close>
+  supply sum_uint64_assn[sepref_fr_rules]
+  unfolding isa_get_saved_pos_def isa_get_saved_pos'_def
+  by sepref
+
+lemma isa_get_saved_pos_get_saved_pos':
+  \<open>(uncurry isa_get_saved_pos', uncurry (RETURN oo get_saved_pos)) \<in>
+    [uncurry get_saved_pos_pre]\<^sub>f
+     \<langle>uint32_nat_rel O arena_el_rel\<rangle>list_rel \<times>\<^sub>f nat_rel \<rightarrow> 
+    \<langle>nat_rel\<rangle>nres_rel\<close>
+  by (intro frefI nres_relI)
+    (auto simp: isa_get_saved_pos_def get_saved_pos_def
+      arena_is_valid_clause_idx_def arena_get_pos_conv isa_get_saved_pos'_def
+      list_rel_imp_same_length get_saved_pos_pre_def
+      intro!: ASSERT_leI)
+
+lemma get_saved_pos_code':
   \<open>(uncurry isa_get_saved_pos_code, uncurry (RETURN \<circ>\<circ> get_saved_pos))
-     \<in> [uncurry get_saved_pos_pre]\<^sub>a arena_assn\<^sup>k *\<^sub>a nat_assn\<^sup>k \<rightarrow> uint32_nat_assn\<close>
-  using isa_get_saved_pos_code.refine[FCOMP isa_get_saved_pos_get_saved_pos]
+     \<in> [uncurry get_saved_pos_pre]\<^sub>a arena_assn\<^sup>k *\<^sub>a nat_assn\<^sup>k \<rightarrow> nat_assn\<close>
+  using isa_get_saved_pos_code.refine[FCOMP isa_get_saved_pos_get_saved_pos']
   unfolding hr_comp_assoc[symmetric] list_rel_compp status_assn_alt_def uncurry_def
   by (auto simp add: arl_assn_comp update_lbd_pre_def)
 
